\documentclass{article}
\usepackage{mathpartir}
\usepackage{amssymb}
\usepackage{biblatex}
\title{\textbf{Bidirectional Typing Rules for Mini}}
\author{Aidan Ewart}

\bibliography{typing}

\addtolength{\topmargin}{-3cm}
\addtolength{\textheight}{3cm}
\begin{document}
\maketitle

Judgements take the conventional bidirectional form of $\Gamma \vdash t \Rightarrow^m \tau$ and $\Gamma \vdash t \Leftarrow^m \tau$.
Otherwise, rules operate in essentially the same manner as \cite{GADT:1}, i.e. we add a 'modifier' $m$, indicating whether the type $\tau$ is 'rigid'.
Similarly to \cite{GADT:1}, we add a function $\Gamma \vdash t \upharpoonleft^m$, which infers the rigidity of the type of $t$.
Note that this does not infer the type of $t$. We also add a commutative function $\lfloor m_1, m_2 \rfloor$, such that $\lfloor r, r \rfloor = r$,
and $\forall x. \lfloor w, x \rfloor = w$, used in inference of the rigidity.

\medskip

\fbox{$ \Gamma \vdash t \Rightarrow^m \tau $}

\begin{mathpar}
    \inferrule[Var]
        { v : \forall \bar{a}. \tau \in \Gamma }
        { \Gamma \vdash v \Rightarrow^m [ \overline{ a \mapsto \upsilon } ] \tau }

    \inferrule[App]
        { \Gamma \vdash f \Rightarrow^w \tau_1 \to \tau_2
        \\ \Gamma \vdash x \Leftarrow^w \tau_1 }
        { \Gamma \vdash \texttt{($f$ $x$)} \Rightarrow^m \tau_2 }

    \inferrule[Abs-Infer]
        { \Gamma, x :^m \tau_1 \vdash t \Leftarrow^m \tau_2 }
        { \Gamma \vdash \texttt{(lam $x$ $t$)} \Rightarrow^m \tau_1 \to \tau_2 }

    \inferrule[Let]
        { \Gamma \vdash u \upharpoonleft^{m_1}
        \\ \Gamma \vdash u \Rightarrow^w \tau_1
        \\ \bar{a} = \mathrm{ftv} ( \tau_1 ) - \mathrm{ftv} ( \Gamma )
        \\ \Gamma, x :^{m_1} \forall \bar{a}. \tau_1 \vdash t \Rightarrow^{m_2} \tau_2 }
        { \Gamma \vdash \texttt{(let ($x$ $u$) $t$)} \Rightarrow^{m_2} \tau_2 }

    \inferrule[Fix]
        { \Gamma \vdash \overline{u_1, u_2 \upharpoonleft^{m_1}}
        \\ \overline{a_1 = \mathrm{ftv} ( \tau_3 ) - \mathrm{ftv} ( \Gamma ) }
        \\ \Gamma,
            \overline{x_1 :^{m_1} \forall a_1. \tau_3},
            \overline{x_2 :^{m_1} \tau_1} \vdash
            \overline{u_1 \Leftarrow^w \forall a_1. \tau_3},
            \overline{u_2 \Leftarrow^w \tau_1},
        \\ \overline{a_2 = \mathrm{ftv} ( \tau_1 ) - \mathrm{ftv} ( \Gamma ) }
        \\ \Gamma,
            \overline{x_1 :^{m_1} \forall a_1. \tau_3},
            \overline{x_2 :^{m_1} \forall a_2. \tau_1} \vdash
            t \Rightarrow^{m_2} \tau_2 }
        { \Gamma \vdash \texttt{(fix $\overline{\texttt{($x_1$ ($u_1$::$\tau_3$))}}$ $\overline{\texttt{($x_2$ $u_2$)}}$ $t$)} \Rightarrow^{m_2} \tau_2 }

    \inferrule[Ann]
        { \bar{a} = \mathrm{ftv}( \tau ) - \mathrm{ftv}( \Gamma )
        \\ \Gamma, \bar{a} \vdash x \Leftarrow^r \tau }
        { \Gamma \vdash \texttt {($x$::$\tau$)} \Rightarrow^m \tau }

    \inferrule[Match]
        { \Gamma \vdash u \upharpoonleft^{m_p}
        \\ \Gamma \vdash u \Rightarrow^w \tau_p
        \\ \Gamma \vdash \overline{\langle p, t \rangle} \Rightarrow^{\langle m_p, m_t, \tau_p \rangle} \tau_t }
        { \Gamma \vdash \texttt{(match $u$ $\overline{\texttt{($p$ -> $t$)}}$)} \Rightarrow^{m_t} \tau_t }

    \inferrule[Lit]
        { L : \tau \in \Gamma }
        { \Gamma \vdash L \Rightarrow^m \tau }
    
    \inferrule[Cons]
        { C : \forall \bar{a}. \bar{\tau_1} \to \bar{\tau_2} \in \Gamma
        \\ \theta = [\overline{a \mapsto \upsilon}] \; \mathrm{ s.t. } \;
        \overline{\Gamma \vdash \theta(v) \Leftarrow^r \tau_1} }
        { \Gamma \vdash C \bar{v} \Rightarrow^m \theta(\tau_2) }

    \inferrule[Primop]
        { O : \bar{\tau_1} \to \tau_2
        \\ \theta = [\overline{a \mapsto \upsilon}] \; \mathrm{ s.t. } \;
        \overline{\Gamma \vdash \theta(v) \Leftarrow^r \tau_1} }
        { \Gamma \vdash O \bar{v} \Rightarrow^m \tau_2 }

\end{mathpar}

\clearpage

\fbox{$ \Gamma \vdash \langle p, t \rangle \Rightarrow^{\langle m_p, m_t, \tau_p \rangle} \tau_t $}

\begin{mathpar}
    \inferrule[PCon-W]
        { C : \forall \bar{a}. \bar{\tau_1} \to T \bar{\tau_2} \in \Gamma
        \\ \theta = [\overline{ a \mapsto \upsilon }] \; \mathrm{ s.t. } \;
        \theta(\bar{\tau_2}) = \bar{\tau_v}
        \\ \Gamma, \overline{v :^w \theta(\tau_v)} \vdash t \Rightarrow^m \tau_t }
        { \Gamma \vdash \langle C \bar{v}, t \rangle \Rightarrow^{\langle w, m, P \bar{\tau_v} \rangle} \tau_t }

    \inferrule[PCon-R]
        { C : \forall \bar{a}. \bar{\tau_1} \to T \bar{\tau_2} \in \Gamma
        \\ \theta = \mathrm{mgu}(\tau_p, \tau_2) 
        \\ \Gamma, \overline{v :^r \theta(\tau_v)} \vdash \theta(t) \Rightarrow^m \theta(\tau_t) }
        { \Gamma \vdash \langle C \bar{v}, t \rangle \Rightarrow^{\langle r, m, P \bar{\tau_v} \rangle} \tau_t }

    \inferrule[PLit]
        { L : \tau_p \in \Gamma 
        \\ \Gamma \vdash t \Rightarrow^{m_t} \tau_t }
        { \Gamma \vdash \langle L, t \rangle \Rightarrow^{\langle m_p, m_t, \tau_p \rangle} \tau_t }
    
    \inferrule[PWild]
        { \Gamma \vdash t \Rightarrow^{m_t} \tau_t }
        { \Gamma \vdash \langle \_, t \rangle \Rightarrow^{\langle m_p, m_t, \tau_p \rangle} \tau_t }

\end{mathpar}

\fbox{$ \Gamma \vdash t \Leftarrow^m \tau $}

\begin{mathpar}
    \inferrule[Abs-Check]
        { \Gamma, x :^m \tau_1 \vdash t \Leftarrow^m \tau_2 }
        { \Gamma \vdash \texttt{(lam $x$ $t$)} \Leftarrow^m \tau_1 \to \tau_2 }

    \inferrule[Check-Infer]
        { \Gamma \vdash t \Rightarrow^m \tau }
        { \Gamma \vdash t \Leftarrow^m \tau }

\end{mathpar}

\fbox{$ \Gamma \vdash t \upharpoonleft^m $}

\begin{mathpar}
    \inferrule[Scr-Var]
        { v \upharpoonleft^m \in \Gamma }
        { \Gamma \vdash v \upharpoonleft^m }
    
    \inferrule[Scr-App]
        { \Gamma \vdash f \upharpoonleft^{m_1}
        \\ \Gamma \vdash x \upharpoonleft^{m_2} }
        { \Gamma \vdash \texttt{($f$ $x$)} \upharpoonleft^{\lfloor m_1, m_2 \rfloor} }

    \inferrule[Scr-Let]
        { \Gamma \vdash u \upharpoonleft^{m_1}
        \\ \Gamma, x \upharpoonleft^{m_1} \vdash t \upharpoonleft^{m_2} }
        { \Gamma \vdash \texttt{(let ($x$ $u$) $t$)} \upharpoonleft^{m_2} }

    \inferrule[Scr-Abs]
        { \Gamma, x \upharpoonleft^w \vdash t \upharpoonleft^{m_1} }
        { \Gamma \vdash \texttt{(lam $x$ $t$)} \upharpoonleft^{m_1} }

    \inferrule[Scr-Ann]
        { }
        { \Gamma \vdash \texttt{($x$::$\tau$)} \upharpoonleft^r }

    \inferrule[Scr-Other]
        { }
        { \Gamma \vdash t \upharpoonleft^w }
\end{mathpar}

\printbibliography

\end{document}
